move more code into head_reductionTheory

examples/lambda/barendregt/head_reductionScript.sml
@@ -1,18 +1,16 @@
-open HolKernel Parse boolLib bossLib
+open HolKernel Parse boolLib bossLib;
 
 open boolSimps relationTheory pred_setTheory listTheory finite_mapTheory
-     hurdUtils;
+     arithmeticTheory pathTheory hurdUtils BasicProvers;
 
 open termTheory appFOLDLTheory chap2Theory chap3Theory nomsetTheory binderLib
-     term_posnsTheory;
+     term_posnsTheory finite_developmentsTheory;
 
 val _ = new_theory "head_reduction"
 
 val _ = ParseExtras.temp_loose_equality()
 
 fun Store_thm(trip as (n,t,tac)) = store_thm trip before export_rewrites [n]
-
-val _ = set_trace "Unicode" 1
 
 Inductive hreduce1 :
   (∀v M N. hreduce1 (LAM v M @@ N) ([N/v]M)) ∧
@@ -211,12 +209,48 @@ val hnf_ccbeta_preserved = store_thm(
     SRW_TAC [][] THEN FULL_SIMP_TAC (srw_ss()) []
   ]);
 
+Theorem hnf_I :
+    hnf I
+Proof
+    RW_TAC std_ss [hnf_thm, I_def]
+QED
+
+Theorem hnf_LAMl[simp] :
+    hnf (LAMl vs M) <=> hnf M
+Proof
+    Induct_on ‘vs’ >> rw []
+QED
+
+Theorem hnf_appstar :
+    !M Ns. hnf (M @* Ns) <=> hnf M /\ (is_abs M ⇒ (Ns = []))
+Proof
+  Induct_on ‘Ns’ using SNOC_INDUCT >> simp[appstar_SNOC] >>
+  dsimp[SF CONJ_ss] >> metis_tac[]
+QED
+
+(* FIXME: can we put ‘ALL_DISTINCT vs’ into RHS? cf. bnf_characterisation *)
+Theorem hnf_cases :
+  !M : term. hnf M <=> ?vs args y. M = LAMl vs (VAR y @* args)
+Proof
+  simp[FORALL_AND_THM, EQ_IMP_THM] >> conj_tac
+  >- (gen_tac >> MP_TAC (Q.SPEC ‘M’ strange_cases)
+      >> RW_TAC std_ss []
+      >- (FULL_SIMP_TAC std_ss [size_1_cases] \\
+          qexistsl_tac [‘vs’, ‘[]’, ‘y’] >> rw [])
+      >> FULL_SIMP_TAC std_ss [hnf_LAMl]
+      >> ‘hnf t /\ ~is_abs t’ by PROVE_TAC [hnf_appstar]
+      >> ‘is_var t’ by METIS_TAC [term_cases]
+      >> FULL_SIMP_TAC std_ss [is_var_cases]
+      >> qexistsl_tac [‘vs’, ‘args’, ‘y’] >> art []) >>
+  simp[PULL_EXISTS, hnf_appstar]
+QED
+
 (* ----------------------------------------------------------------------
     Weak head reductions (weak_head or -w->)
    ---------------------------------------------------------------------- *)
 
 Inductive weak_head :
-  (∀v M N. weak_head (LAM v M @@ N) ([N/v]M)) ∧
+  (∀v M N :term. weak_head (LAM v M @@ N) ([N/v]M)) ∧
   (∀M₁ M₂ N. weak_head M₁ M₂ ⇒ weak_head (M₁ @@ N) (M₂ @@ N))
 End
 
@@ -540,45 +574,272 @@ val is_head_redex_vsubst_invariant = store_thm(
   HO_MATCH_MP_TAC nc_INDUCTION2 THEN Q.EXISTS_TAC `{x;v}` THEN
   SRW_TAC [][is_head_redex_thm, SUB_THM, SUB_VAR]);
 
-(* ----------------------------------------------------------------------
-    More results about head normal forms (hnf)
-   ---------------------------------------------------------------------- *)
+val head_redex_preserved = store_thm(
+  "head_redex_preserved",
+  ``!M p N.
+      labelled_redn beta M p N ==>
+      !h. h is_head_redex M /\ ~(h = p) ==> h is_head_redex N``,
+  HO_MATCH_MP_TAC strong_labelled_redn_ind THEN
+  SRW_TAC [][is_head_redex_thm, beta_def] THENL [
+    FULL_SIMP_TAC (srw_ss()) [is_head_redex_thm],
+    `?v t. M = LAM v t` by PROVE_TAC [is_abs_thm, term_CASES] THEN
+    FULL_SIMP_TAC (srw_ss()) [labelled_redn_lam],
+    `?f x. M = f @@ x` by PROVE_TAC [is_comb_APP_EXISTS] THEN
+    SRW_TAC [][] THEN
+    Q.PAT_X_ASSUM `labelled_redn beta _ _ _` MP_TAC THEN
+    ONCE_REWRITE_TAC [labelled_redn_cases] THEN
+    FULL_SIMP_TAC (srw_ss()) [is_head_redex_thm, beta_def] THEN
+    PROVE_TAC [is_comb_thm]
+  ]);
 
-Theorem hnf_I :
-    hnf I
+val is_head_reduction_def = Define`
+  is_head_reduction s = okpath (labelled_redn beta) s /\
+                        !i. i + 1 IN PL s ==>
+                            nth_label i s is_head_redex el i s
+`;
+
+Theorem is_head_reduction_thm[simp] :
+    (is_head_reduction (stopped_at x) = T) /\
+    (is_head_reduction (pcons x r p) =
+       labelled_redn beta x r (first p) /\ r is_head_redex x /\
+       is_head_reduction p)
 Proof
-    RW_TAC std_ss [hnf_thm, I_def]
+  SRW_TAC [][is_head_reduction_def, GSYM ADD1,
+             EQ_IMP_THM]
+  THENL [
+    POP_ASSUM (Q.SPEC_THEN `0` MP_TAC) THEN SRW_TAC [][],
+    RES_TAC THEN FULL_SIMP_TAC (srw_ss()) [],
+    Cases_on `i` THEN SRW_TAC [][]
+  ]
 QED
 
-Theorem hnf_LAMl[simp] :
-    hnf (LAMl vs M) <=> hnf M
-Proof
-    Induct_on ‘vs’ >> rw []
-QED
+val _ = add_infix ("head_reduces", 760, NONASSOC)
+val head_reduces_def = Define`
+  M head_reduces N = ?s. finite s /\ (first s = M) /\ (last s = N) /\
+                         is_head_reduction s
+`;
 
-Theorem hnf_appstar :
-    !M Ns. hnf (M @* Ns) <=> hnf M /\ (is_abs M ⇒ (Ns = []))
-Proof
-  Induct_on ‘Ns’ using SNOC_INDUCT >> simp[appstar_SNOC] >>
-  dsimp[SF CONJ_ss] >> metis_tac[]
-QED
 
-(* FIXME: can we put ‘ALL_DISTINCT vs’ into RHS? cf. bnf_characterisation *)
-Theorem hnf_cases :
-  !M : term. hnf M <=> ?vs args y. M = LAMl vs (VAR y @* args)
-Proof
-  simp[FORALL_AND_THM, EQ_IMP_THM] >> conj_tac
-  >- (gen_tac >> MP_TAC (Q.SPEC ‘M’ strange_cases)
-      >> RW_TAC std_ss []
-      >- (FULL_SIMP_TAC std_ss [size_1_cases] \\
-          qexistsl_tac [‘vs’, ‘[]’, ‘y’] >> rw [])
-      >> FULL_SIMP_TAC std_ss [hnf_LAMl]
-      >> ‘hnf t /\ ~is_abs t’ by PROVE_TAC [hnf_appstar]
-      >> ‘is_var t’ by METIS_TAC [term_cases]
-      >> FULL_SIMP_TAC std_ss [is_var_cases]
-      >> qexistsl_tac [‘vs’, ‘args’, ‘y’] >> art []) >>
-  simp[PULL_EXISTS, hnf_appstar]
-QED
+val head_reduce1_def = store_thm(
+  "head_reduce1_def",
+  ``M -h-> N = (?r. r is_head_redex M /\ labelled_redn beta M r N)``,
+  EQ_TAC THENL [
+    Q_TAC SUFF_TAC `!M N. M -h-> N ==>
+                          ?r. r is_head_redex M /\ labelled_redn beta M r N`
+          THEN1 METIS_TAC [] THEN
+    HO_MATCH_MP_TAC hreduce1_ind THEN SRW_TAC [][] THENL [
+      METIS_TAC [beta_def, is_head_redex_rules, labelled_redn_rules],
+      METIS_TAC [is_head_redex_rules, labelled_redn_rules],
+      Q.SPEC_THEN `M` FULL_STRUCT_CASES_TAC term_CASES THENL [
+        FULL_SIMP_TAC (srw_ss()) [Once labelled_redn_cases, beta_def],
+        METIS_TAC [is_head_redex_rules, labelled_redn_rules],
+        FULL_SIMP_TAC (srw_ss()) []
+      ]
+    ],
+    Q_TAC SUFF_TAC `!M r N. labelled_redn beta M r N ==>
+                            r is_head_redex M ==> M -h-> N`
+          THEN1 METIS_TAC [] THEN
+    HO_MATCH_MP_TAC labelled_redn_ind THEN
+    SIMP_TAC (srw_ss() ++ DNF_ss) [beta_def, is_head_redex_thm,
+                                   Once is_comb_APP_EXISTS, hreduce1_rwts]
+  ]);
+
+val head_reduces_RTC_hreduce1 = store_thm(
+  "head_reduces_RTC_hreduce1",
+  ``(head_reduces) = RTC (-h->)``,
+  SIMP_TAC (srw_ss()) [head_reduces_def, FUN_EQ_THM, GSYM LEFT_FORALL_IMP_THM,
+                       FORALL_AND_THM, EQ_IMP_THM] THEN
+  CONJ_TAC THENL [
+    Q_TAC SUFF_TAC `!s. finite s ==>
+                        is_head_reduction s ==>
+                        RTC (-h->) (first s) (last s)` THEN1
+          PROVE_TAC [] THEN
+    HO_MATCH_MP_TAC pathTheory.finite_path_ind THEN
+    SIMP_TAC (srw_ss()) [relationTheory.RTC_RULES] THEN
+    MAP_EVERY Q.X_GEN_TAC [`x`,`r`,`p`] THEN REPEAT STRIP_TAC THEN
+    MATCH_MP_TAC (CONJUNCT2 (SPEC_ALL relationTheory.RTC_RULES)) THEN
+    Q.EXISTS_TAC `first p` THEN SRW_TAC [][head_reduce1_def] THEN
+    PROVE_TAC [],
+    HO_MATCH_MP_TAC relationTheory.RTC_INDUCT THEN
+    SRW_TAC [][head_reduce1_def] THENL [
+      Q.EXISTS_TAC `stopped_at x` THEN SRW_TAC [][],
+      Q.EXISTS_TAC `pcons x r s` THEN SRW_TAC [][]
+    ]
+  ]);
+
+val head_reduces_reduction_beta = store_thm(
+  "head_reduces_reduction_beta",
+  ``!M N. M head_reduces N ==> reduction beta M N``,
+  SIMP_TAC (srw_ss()) [head_reduces_RTC_hreduce1] THEN
+  MATCH_MP_TAC relationTheory.RTC_MONOTONE THEN
+  METIS_TAC [head_reduce1_def, labelled_redn_cc]);
+
+val head_reduces_TRANS = store_thm(
+  "head_reduces_TRANS",
+  ``!M N P. M head_reduces N /\ N head_reduces P ==> M head_reduces P``,
+  METIS_TAC [relationTheory.RTC_RTC, head_reduces_RTC_hreduce1]);
+
+val has_hnf_def = Define`
+  has_hnf M = ?N. M == N /\ hnf N
+`;
+
+val has_bnf_hnf = store_thm(
+  "has_bnf_hnf",
+  ``has_bnf M ⇒ has_hnf M``,
+  SRW_TAC [][has_hnf_def, chap2Theory.has_bnf_def] THEN
+  METIS_TAC [bnf_hnf]);
+
+val head_reduct_def = Define`
+  head_reduct M = if ?r. r is_head_redex M then
+                    SOME (@N. M -h-> N)
+                  else NONE
+`;
+
+val head_reduct_unique = store_thm(
+  "head_reduct_unique",
+  ``!M N. M -h-> N ==> (head_reduct M = SOME N)``,
+  SRW_TAC [][head_reduce1_def, head_reduct_def] THEN1 METIS_TAC [] THEN
+  SELECT_ELIM_TAC THEN METIS_TAC [is_head_redex_unique, labelled_redn_det]);
+
+val head_reduct_NONE = store_thm(
+  "head_reduct_NONE",
+  ``(head_reduct M = NONE) = !N. ~(M -h-> N)``,
+  SRW_TAC [][head_reduct_def, head_reduce1_def] THEN
+  METIS_TAC [head_redex_is_redex, IN_term_IN_redex_posns,
+             is_redex_occurrence_def]);
+
+val head_reduct_SOME = store_thm(
+  "head_reduct_SOME",
+  ``(head_reduct M = SOME N) = M -h-> N``,
+  SIMP_TAC (srw_ss()) [EQ_IMP_THM, head_reduct_unique] THEN
+  SRW_TAC [][head_reduct_def] THEN SELECT_ELIM_TAC THEN
+  SRW_TAC [][head_reduce1_def] THEN
+  METIS_TAC [head_redex_is_redex, IN_term_IN_redex_posns,
+             is_redex_occurrence_def]);
+
+val drop_not_stopped = prove(
+  ``!i p. SUC i IN PL p ==> ?v r q. drop i p = pcons v r q``,
+  Induct THEN GEN_TAC THEN
+  Q.SPEC_THEN `p` STRUCT_CASES_TAC path_cases THEN
+  SRW_TAC [][]);
+
+val drop_tail_commute = store_thm(
+  "drop_tail_commute",
+  ``!i p. SUC i IN PL p ==> (drop i (tail p) = tail (drop i p))``,
+  Induct THEN SIMP_TAC (srw_ss()) [Once FORALL_path] THEN
+  SRW_TAC [][]);
+
+val is_head_reduction_coind = store_thm(
+  "is_head_reduction_coind",
+  ``(!x r q. P (pcons x r q) ==>
+             labelled_redn beta x r (first q) /\
+             r is_head_redex x /\ P q) ==>
+    !p. P p ==> is_head_reduction p``,
+  SIMP_TAC (srw_ss()) [is_head_reduction_def, IMP_CONJ_THM,
+                       FORALL_AND_THM] THEN CONJ_TAC
+  THENL [
+    STRIP_TAC THEN HO_MATCH_MP_TAC okpath_co_ind THEN METIS_TAC [],
+    STRIP_TAC THEN GEN_TAC THEN STRIP_TAC THEN
+    Q_TAC SUFF_TAC `!i. i + 1 IN PL p ==> nth_label i p is_head_redex el i p /\
+                                          P (drop (i + 1) p)` THEN1
+          METIS_TAC [] THEN
+    Induct THEN FULL_SIMP_TAC (srw_ss()) [GSYM ADD1] THENL [
+      Q.ISPEC_THEN `p` FULL_STRUCT_CASES_TAC path_cases THEN
+      FULL_SIMP_TAC (srw_ss()) [] THEN METIS_TAC [],
+      STRIP_TAC THEN
+      `SUC i IN PL p`
+         by METIS_TAC [PL_downward_closed, DECIDE ``x < SUC x``] THEN
+      FULL_SIMP_TAC (srw_ss()) [] THEN
+      Q.ISPEC_THEN `p` FULL_STRUCT_CASES_TAC path_cases THEN
+      FULL_SIMP_TAC (srw_ss()) [] THEN
+      `?y s q'. drop i q = pcons y s q'` by METIS_TAC [drop_not_stopped] THEN
+      `labelled_redn beta y s (first q') /\ s is_head_redex y /\ P q'`
+          by METIS_TAC [stopped_at_not_pcons, pcons_11] THEN
+      `el 0 (drop i q) = el i q` by SRW_TAC [][] THEN
+      `el i q = y` by METIS_TAC [el_def, first_thm] THEN
+      `nth_label 0 (drop i q) = nth_label i q` by SRW_TAC [][] THEN
+      `nth_label i q = s` by METIS_TAC [nth_label_def, first_label_def] THEN
+      SRW_TAC [][drop_tail_commute]
+    ]
+  ]);
+
+val head_reduction_path_uexists = prove(
+  ``!M. ?!p. (first p = M) /\ is_head_reduction p /\
+             (finite p ==> hnf (last p))``,
+  GEN_TAC THEN
+  Q.ISPEC_THEN `\M. (M, OPTION_MAP (\N. ((@r. r is_head_redex M), N))
+                                  (head_reduct M))`
+               STRIP_ASSUME_TAC path_Axiom THEN
+  `!M. first (g M) = M`
+      by (POP_ASSUM (fn th => SRW_TAC [][Once th]) THEN
+          Cases_on `head_reduct M` THEN SRW_TAC [][]) THEN
+  `!M. is_head_reduction (g M)`
+      by (Q_TAC SUFF_TAC
+                `!p. (?M. p = g M) ==> is_head_reduction p` THEN1
+                METIS_TAC [] THEN
+          HO_MATCH_MP_TAC is_head_reduction_coind THEN
+          Q.PAT_X_ASSUM `!x:term. g x = Z`
+                          (fn th => SIMP_TAC (srw_ss())
+                                             [Once th, SimpL ``(==>)``]) THEN
+          REPEAT GEN_TAC THEN STRIP_TAC THEN
+          Cases_on `head_reduct M` THEN
+          FULL_SIMP_TAC (srw_ss()) [head_reduct_SOME, head_reduce1_def] THEN
+          REPEAT VAR_EQ_TAC THEN SELECT_ELIM_TAC THEN
+          METIS_TAC [is_head_redex_unique]) THEN
+  `!p. finite p ==> !M. (p = g M) ==> hnf (last p)`
+      by (HO_MATCH_MP_TAC finite_path_ind THEN
+          SIMP_TAC (srw_ss()) [] THEN CONJ_TAC THEN REPEAT GEN_TAC THENL [
+            Q.PAT_X_ASSUM `!x:term. g x = Z`
+                        (fn th => ONCE_REWRITE_TAC [th]) THEN
+            Cases_on `head_reduct M` THEN SRW_TAC [][] THEN
+            FULL_SIMP_TAC (srw_ss()) [hnf_no_head_redex, head_reduct_NONE,
+                                      head_reduce1_def] THEN
+            METIS_TAC [head_redex_is_redex, IN_term_IN_redex_posns,
+                       is_redex_occurrence_def],
+            STRIP_TAC THEN GEN_TAC THEN
+            Q.PAT_X_ASSUM `!x:term. g x = Z`
+                        (fn th => ONCE_REWRITE_TAC [th]) THEN
+            Cases_on `head_reduct M` THEN SRW_TAC [][]
+          ]) THEN
+  SIMP_TAC (srw_ss()) [EXISTS_UNIQUE_THM] THEN CONJ_TAC THENL [
+    Q.EXISTS_TAC `g M` THEN
+    Q.PAT_X_ASSUM `!x:term. g x = Z` (K ALL_TAC) THEN METIS_TAC [],
+    REPEAT (POP_ASSUM (K ALL_TAC)) THEN
+    REPEAT STRIP_TAC THEN
+    ONCE_REWRITE_TAC [path_bisimulation] THEN
+    Q.EXISTS_TAC `\p1 p2. is_head_reduction p1 /\ is_head_reduction p2 /\
+                          (first p1 = first p2) /\
+                          (finite p1 ==> hnf (last p1)) /\
+                          (finite p2 ==> hnf (last p2))` THEN
+    SRW_TAC [][] THEN
+    Q.ISPEC_THEN `q1` (REPEAT_TCL STRIP_THM_THEN SUBST_ALL_TAC)
+                 path_cases THEN
+    Q.ISPEC_THEN `q2` (REPEAT_TCL STRIP_THM_THEN SUBST_ALL_TAC)
+                 path_cases THEN FULL_SIMP_TAC (srw_ss()) []
+    THENL [
+      METIS_TAC [hnf_no_head_redex],
+      METIS_TAC [hnf_no_head_redex],
+      METIS_TAC [is_head_redex_unique, labelled_redn_det]
+    ]
+  ]);
+
+val head_reduction_path_def = new_specification(
+  "head_reduction_path_def",
+  ["head_reduction_path"],
+  CONJUNCT1 ((SIMP_RULE bool_ss [EXISTS_UNIQUE_THM] o
+              SIMP_RULE bool_ss [UNIQUE_SKOLEM_THM])
+             head_reduction_path_uexists));
+
+val head_reduction_path_unique = store_thm(
+  "head_reduction_path_unique",
+  ``!M p. (first p = M) /\ is_head_reduction p /\
+          (finite p ==> hnf (last p)) ==>
+          (head_reduction_path M = p)``,
+  REPEAT STRIP_TAC THEN
+  Q.SPEC_THEN `M` (ASSUME_TAC o CONJUNCT2 o
+                   SIMP_RULE bool_ss [EXISTS_UNIQUE_THM])
+              head_reduction_path_uexists THEN
+  METIS_TAC [head_reduction_path_def]);
 
 val _ = export_theory()
 val _ = html_theory "head_reduction";
