examples/lambda/barendregt/standardisationScript.sml
@@ -26,10 +26,6 @@ val _ = ParseExtras.temp_loose_equality()
 val RUNION_def = relationTheory.RUNION
 val ADD1 = arithmeticTheory.ADD1
 
-
-
-fun Store_Thm(n,t,tac) = store_thm(n,t,tac) before export_rewrites [n]
-
 (* Section 11.4 of Barendregt *)
 
 val standard_reduction_def = Define`
@@ -67,12 +63,13 @@ val is_internal_redex_def = Define`
   p is_internal_redex t = ~(p is_head_redex t) /\ p IN redex_posns t
 `;
 
-val NIL_never_internal_redex = Store_Thm(
-  "NIL_never_internal_redex",
-  ``!t. ~([] is_internal_redex t)``,
+Theorem NIL_never_internal_redex[simp] :
+    !t. ~([] is_internal_redex t)
+Proof
   GEN_TAC THEN
   Q.SPEC_THEN `t` STRUCT_CASES_TAC term_CASES THEN
-  SRW_TAC [][is_internal_redex_def, is_head_redex_thm, redex_posns_thm]);
+  SRW_TAC [][is_internal_redex_def, is_head_redex_thm, redex_posns_thm]
+QED
 
 val _ = add_infix("i_reduces", 760, NONASSOC)
 (* definition 11.4.2 (ii) *)
@@ -132,24 +129,7 @@ val i1_reduces_def = Define`
                        ?FS. s IN complete_development M FS
 `;
 
-val head_redex_preserved = store_thm(
-  "head_redex_preserved",
-  ``!M p N.
-      labelled_redn beta M p N ==>
-      !h. h is_head_redex M /\ ~(h = p) ==> h is_head_redex N``,
-  HO_MATCH_MP_TAC strong_labelled_redn_ind THEN
-  SRW_TAC [][is_head_redex_thm, beta_def] THENL [
-    FULL_SIMP_TAC (srw_ss()) [is_head_redex_thm],
-    `?v t. M = LAM v t` by PROVE_TAC [is_abs_thm, term_CASES] THEN
-    FULL_SIMP_TAC (srw_ss()) [labelled_redn_lam],
-    `?f x. M = f @@ x` by PROVE_TAC [is_comb_APP_EXISTS] THEN
-    SRW_TAC [][] THEN
-    Q.PAT_X_ASSUM `labelled_redn beta _ _ _` MP_TAC THEN
-    ONCE_REWRITE_TAC [labelled_redn_cases] THEN
-    FULL_SIMP_TAC (srw_ss()) [is_head_redex_thm, beta_def] THEN
-    PROVE_TAC [is_comb_thm]
-  ]);
-
+(* NOTE: the antecedent ‘delta is_internal_redex M’ is unnecessary *)
 val lemma11_4_3i = store_thm(
   "lemma11_4_3i",
   ``!M delta N.
@@ -498,89 +478,6 @@ val lemma11_4_3iii = store_thm(
     ]
   ]);
 
-val is_head_reduction_def = Define`
-  is_head_reduction s = okpath (labelled_redn beta) s /\
-                        !i. i + 1 IN PL s ==>
-                            nth_label i s is_head_redex el i s
-`;
-
-val is_head_reduction_thm = store_thm(
-  "is_head_reduction_thm",
-  ``(is_head_reduction (stopped_at x) = T) /\
-    (is_head_reduction (pcons x r p) =
-       labelled_redn beta x r (first p) /\ r is_head_redex x /\
-       is_head_reduction p)``,
-  SRW_TAC [][is_head_reduction_def, GSYM ADD1,
-             EQ_IMP_THM]
-  THENL [
-    POP_ASSUM (Q.SPEC_THEN `0` MP_TAC) THEN SRW_TAC [][],
-    RES_TAC THEN FULL_SIMP_TAC (srw_ss()) [],
-    Cases_on `i` THEN SRW_TAC [][]
-  ]);
-val _ = export_rewrites ["is_head_reduction_thm"]
-
-
-val _ = add_infix ("head_reduces", 760, NONASSOC)
-val head_reduces_def = Define`
-  M head_reduces N = ?s. finite s /\ (first s = M) /\ (last s = N) /\
-                         is_head_reduction s
-`;
-
-
-val head_reduce1_def = store_thm(
-  "head_reduce1_def",
-  ``M -h-> N = (?r. r is_head_redex M /\ labelled_redn beta M r N)``,
-  EQ_TAC THENL [
-    Q_TAC SUFF_TAC `!M N. M -h-> N ==>
-                          ?r. r is_head_redex M /\ labelled_redn beta M r N`
-          THEN1 METIS_TAC [] THEN
-    HO_MATCH_MP_TAC hreduce1_ind THEN SRW_TAC [][] THENL [
-      METIS_TAC [beta_def, is_head_redex_rules, labelled_redn_rules],
-      METIS_TAC [is_head_redex_rules, labelled_redn_rules],
-      Q.SPEC_THEN `M` FULL_STRUCT_CASES_TAC term_CASES THENL [
-        FULL_SIMP_TAC (srw_ss()) [Once labelled_redn_cases, beta_def],
-        METIS_TAC [is_head_redex_rules, labelled_redn_rules],
-        FULL_SIMP_TAC (srw_ss()) []
-      ]
-    ],
-    Q_TAC SUFF_TAC `!M r N. labelled_redn beta M r N ==>
-                            r is_head_redex M ==> M -h-> N`
-          THEN1 METIS_TAC [] THEN
-    HO_MATCH_MP_TAC labelled_redn_ind THEN
-    SIMP_TAC (srw_ss() ++ DNF_ss) [beta_def, is_head_redex_thm,
-                                   Once is_comb_APP_EXISTS, hreduce1_rwts]
-  ]);
-
-val head_reduces_RTC_hreduce1 = store_thm(
-  "head_reduces_RTC_hreduce1",
-  ``(head_reduces) = RTC (-h->)``,
-  SIMP_TAC (srw_ss()) [head_reduces_def, FUN_EQ_THM, GSYM LEFT_FORALL_IMP_THM,
-                       FORALL_AND_THM, EQ_IMP_THM] THEN
-  CONJ_TAC THENL [
-    Q_TAC SUFF_TAC `!s. finite s ==>
-                        is_head_reduction s ==>
-                        RTC (-h->) (first s) (last s)` THEN1
-          PROVE_TAC [] THEN
-    HO_MATCH_MP_TAC pathTheory.finite_path_ind THEN
-    SIMP_TAC (srw_ss()) [relationTheory.RTC_RULES] THEN
-    MAP_EVERY Q.X_GEN_TAC [`x`,`r`,`p`] THEN REPEAT STRIP_TAC THEN
-    MATCH_MP_TAC (CONJUNCT2 (SPEC_ALL relationTheory.RTC_RULES)) THEN
-    Q.EXISTS_TAC `first p` THEN SRW_TAC [][head_reduce1_def] THEN
-    PROVE_TAC [],
-    HO_MATCH_MP_TAC relationTheory.RTC_INDUCT THEN
-    SRW_TAC [][head_reduce1_def] THENL [
-      Q.EXISTS_TAC `stopped_at x` THEN SRW_TAC [][],
-      Q.EXISTS_TAC `pcons x r s` THEN SRW_TAC [][]
-    ]
-  ]);
-
-val head_reduces_reduction_beta = store_thm(
-  "head_reduces_reduction_beta",
-  ``!M N. M head_reduces N ==> reduction beta M N``,
-  SIMP_TAC (srw_ss()) [head_reduces_RTC_hreduce1] THEN
-  MATCH_MP_TAC relationTheory.RTC_MONOTONE THEN
-  METIS_TAC [head_reduce1_def, labelled_redn_cc]);
-
 val beta0_induction =
     REWRITE_RULE [relationTheory.inv_DEF]
                  (MATCH_MP relationTheory.WF_INDUCTION_THM prop11_2_20)
@@ -612,10 +509,9 @@ val lrcc_monotone = store_thm(
   REPEAT GEN_TAC THEN STRIP_TAC THEN
   HO_MATCH_MP_TAC lrcc_ind THEN PROVE_TAC [lrcc_rules]);
 
-
-val length_lift_path = Store_Thm(
-  "length_lift_path",
-  ``!M p. length (lift_path M p) = length p``,
+Theorem length_lift_path[simp] :
+    !M p. length (lift_path M p) = length p
+Proof
   REPEAT GEN_TAC THEN
   Cases_on `finite p` THENL [
     Q.ID_SPEC_TAC `M` THEN POP_ASSUM MP_TAC THEN
@@ -623,7 +519,8 @@ val length_lift_path = Store_Thm(
     HO_MATCH_MP_TAC pathTheory.finite_path_ind THEN
     SRW_TAC [][lift_path_def, pathTheory.length_thm, finite_lift_path],
     SRW_TAC [][pathTheory.length_def, finite_lift_path]
-  ]);
+  ]
+QED
 
 val PL_lift_path = store_thm(
   "PL_lift_path",
@@ -671,10 +568,11 @@ val zero_vsubst = store_thm(
   SRW_TAC [][zero_def, GSYM nlabel_vsubst_commutes, n_posns_vsubst_invariant,
              strip_label_vsubst_commutes]);
 
-val FV_zero = Store_Thm(
-  "FV_zero",
-  ``FV (zero n t) = FV t``,
-  SRW_TAC [][zero_def, FV_nlabel, FV_strip_label]);
+Theorem FV_zero[simp] :
+    FV (zero n t) = FV t
+Proof
+  SRW_TAC [][zero_def, FV_nlabel, FV_strip_label]
+QED
 
 val zero_subst = store_thm(
   "zero_subst",
@@ -917,11 +815,6 @@ val i1_reduces_i_reduces = prove(
 val _ = augment_srw_ss [rewrites [REWRITE_CONV [EMPTY_SUBSET,
                                                 redex_occurrences_SUBSET]
                                   ``{} SUBSET (M:term)``]]
-
-val head_reduces_TRANS = store_thm(
-  "head_reduces_TRANS",
-  ``!M N P. M head_reduces N /\ N head_reduces P ==> M head_reduces P``,
-  METIS_TAC [relationTheory.RTC_RTC, head_reduces_RTC_hreduce1]);
 
 val lemma11_4_5 = store_thm(
   "lemma11_4_5",
@@ -1238,12 +1131,12 @@ val i_reduces_to_LAMl = prove(
     PROVE_TAC [relationTheory.RTC_RULES, i_reduce1_under_LAMl]
   ]);
 
-val size_vsubst = Store_Thm(
-  "size_vsubst",
-  ``!M:term. size ([VAR v/u] M) = size M``,
+Theorem size_vsubst[simp] :
+    !M:term. size ([VAR v/u] M) = size M
+Proof
   HO_MATCH_MP_TAC nc_INDUCTION2 THEN Q.EXISTS_TAC `{u;v}` THEN
-  SRW_TAC [][SUB_VAR, SUB_THM]);
-
+  SRW_TAC [][SUB_VAR, SUB_THM]
+QED
 
 val size_ISUB = prove(
   ``!R N:term. RENAMING R ==> (size (N ISUB R) = size N)``,
@@ -1930,168 +1823,6 @@ val standardisation_theorem = store_thm(
     SRW_TAC [][head_standard_is_standard]
   ]);
 
-val has_hnf_def = Define`
-  has_hnf M = ?N. M == N /\ hnf N
-`;
-
-val has_bnf_hnf = store_thm(
-  "has_bnf_hnf",
-  ``has_bnf M ⇒ has_hnf M``,
-  SRW_TAC [][has_hnf_def, chap2Theory.has_bnf_def] THEN
-  METIS_TAC [bnf_hnf]);
-
-val head_reduct_def = Define`
-  head_reduct M = if ?r. r is_head_redex M then
-                    SOME (@N. M -h-> N)
-                  else NONE
-`;
-
-val head_reduct_unique = store_thm(
-  "head_reduct_unique",
-  ``!M N. M -h-> N ==> (head_reduct M = SOME N)``,
-  SRW_TAC [][head_reduce1_def, head_reduct_def] THEN1 METIS_TAC [] THEN
-  SELECT_ELIM_TAC THEN METIS_TAC [is_head_redex_unique, labelled_redn_det]);
-
-val head_reduct_NONE = store_thm(
-  "head_reduct_NONE",
-  ``(head_reduct M = NONE) = !N. ~(M -h-> N)``,
-  SRW_TAC [][head_reduct_def, head_reduce1_def] THEN
-  METIS_TAC [head_redex_is_redex, IN_term_IN_redex_posns,
-             is_redex_occurrence_def]);
-
-val head_reduct_SOME = store_thm(
-  "head_reduct_SOME",
-  ``(head_reduct M = SOME N) = M -h-> N``,
-  SIMP_TAC (srw_ss()) [EQ_IMP_THM, head_reduct_unique] THEN
-  SRW_TAC [][head_reduct_def] THEN SELECT_ELIM_TAC THEN
-  SRW_TAC [][head_reduce1_def] THEN
-  METIS_TAC [head_redex_is_redex, IN_term_IN_redex_posns,
-             is_redex_occurrence_def]);
-
-val drop_not_stopped = prove(
-  ``!i p. SUC i IN PL p ==> ?v r q. drop i p = pcons v r q``,
-  Induct THEN GEN_TAC THEN
-  Q.SPEC_THEN `p` STRUCT_CASES_TAC path_cases THEN
-  SRW_TAC [][]);
-
-val drop_tail_commute = store_thm(
-  "drop_tail_commute",
-  ``!i p. SUC i IN PL p ==> (drop i (tail p) = tail (drop i p))``,
-  Induct THEN SIMP_TAC (srw_ss()) [Once FORALL_path] THEN
-  SRW_TAC [][]);
-
-val is_head_reduction_coind = store_thm(
-  "is_head_reduction_coind",
-  ``(!x r q. P (pcons x r q) ==>
-             labelled_redn beta x r (first q) /\
-             r is_head_redex x /\ P q) ==>
-    !p. P p ==> is_head_reduction p``,
-  SIMP_TAC (srw_ss()) [is_head_reduction_def, IMP_CONJ_THM,
-                       FORALL_AND_THM] THEN CONJ_TAC
-  THENL [
-    STRIP_TAC THEN HO_MATCH_MP_TAC okpath_co_ind THEN METIS_TAC [],
-    STRIP_TAC THEN GEN_TAC THEN STRIP_TAC THEN
-    Q_TAC SUFF_TAC `!i. i + 1 IN PL p ==> nth_label i p is_head_redex el i p /\
-                                          P (drop (i + 1) p)` THEN1
-          METIS_TAC [] THEN
-    Induct THEN FULL_SIMP_TAC (srw_ss()) [GSYM ADD1] THENL [
-      Q.ISPEC_THEN `p` FULL_STRUCT_CASES_TAC path_cases THEN
-      FULL_SIMP_TAC (srw_ss()) [] THEN METIS_TAC [],
-      STRIP_TAC THEN
-      `SUC i IN PL p`
-         by METIS_TAC [PL_downward_closed, DECIDE ``x < SUC x``] THEN
-      FULL_SIMP_TAC (srw_ss()) [] THEN
-      Q.ISPEC_THEN `p` FULL_STRUCT_CASES_TAC path_cases THEN
-      FULL_SIMP_TAC (srw_ss()) [] THEN
-      `?y s q'. drop i q = pcons y s q'` by METIS_TAC [drop_not_stopped] THEN
-      `labelled_redn beta y s (first q') /\ s is_head_redex y /\ P q'`
-          by METIS_TAC [stopped_at_not_pcons, pcons_11] THEN
-      `el 0 (drop i q) = el i q` by SRW_TAC [][] THEN
-      `el i q = y` by METIS_TAC [el_def, first_thm] THEN
-      `nth_label 0 (drop i q) = nth_label i q` by SRW_TAC [][] THEN
-      `nth_label i q = s` by METIS_TAC [nth_label_def, first_label_def] THEN
-      SRW_TAC [][drop_tail_commute]
-    ]
-  ]);
-
-val head_reduction_path_uexists = prove(
-  ``!M. ?!p. (first p = M) /\ is_head_reduction p /\
-             (finite p ==> hnf (last p))``,
-  GEN_TAC THEN
-  Q.ISPEC_THEN `\M. (M, OPTION_MAP (\N. ((@r. r is_head_redex M), N))
-                                  (head_reduct M))`
-               STRIP_ASSUME_TAC path_Axiom THEN
-  `!M. first (g M) = M`
-      by (POP_ASSUM (fn th => SRW_TAC [][Once th]) THEN
-          Cases_on `head_reduct M` THEN SRW_TAC [][]) THEN
-  `!M. is_head_reduction (g M)`
-      by (Q_TAC SUFF_TAC
-                `!p. (?M. p = g M) ==> is_head_reduction p` THEN1
-                METIS_TAC [] THEN
-          HO_MATCH_MP_TAC is_head_reduction_coind THEN
-          Q.PAT_X_ASSUM `!x:term. g x = Z`
-                          (fn th => SIMP_TAC (srw_ss())
-                                             [Once th, SimpL ``(==>)``]) THEN
-          REPEAT GEN_TAC THEN STRIP_TAC THEN
-          Cases_on `head_reduct M` THEN
-          FULL_SIMP_TAC (srw_ss()) [head_reduct_SOME, head_reduce1_def] THEN
-          REPEAT VAR_EQ_TAC THEN SELECT_ELIM_TAC THEN
-          METIS_TAC [is_head_redex_unique]) THEN
-  `!p. finite p ==> !M. (p = g M) ==> hnf (last p)`
-      by (HO_MATCH_MP_TAC finite_path_ind THEN
-          SIMP_TAC (srw_ss()) [] THEN CONJ_TAC THEN REPEAT GEN_TAC THENL [
-            Q.PAT_X_ASSUM `!x:term. g x = Z`
-                        (fn th => ONCE_REWRITE_TAC [th]) THEN
-            Cases_on `head_reduct M` THEN SRW_TAC [][] THEN
-            FULL_SIMP_TAC (srw_ss()) [hnf_no_head_redex, head_reduct_NONE,
-                                      head_reduce1_def] THEN
-            METIS_TAC [head_redex_is_redex, IN_term_IN_redex_posns,
-                       is_redex_occurrence_def],
-            STRIP_TAC THEN GEN_TAC THEN
-            Q.PAT_X_ASSUM `!x:term. g x = Z`
-                        (fn th => ONCE_REWRITE_TAC [th]) THEN
-            Cases_on `head_reduct M` THEN SRW_TAC [][]
-          ]) THEN
-  SIMP_TAC (srw_ss()) [EXISTS_UNIQUE_THM] THEN CONJ_TAC THENL [
-    Q.EXISTS_TAC `g M` THEN
-    Q.PAT_X_ASSUM `!x:term. g x = Z` (K ALL_TAC) THEN METIS_TAC [],
-    REPEAT (POP_ASSUM (K ALL_TAC)) THEN
-    REPEAT STRIP_TAC THEN
-    ONCE_REWRITE_TAC [path_bisimulation] THEN
-    Q.EXISTS_TAC `\p1 p2. is_head_reduction p1 /\ is_head_reduction p2 /\
-                          (first p1 = first p2) /\
-                          (finite p1 ==> hnf (last p1)) /\
-                          (finite p2 ==> hnf (last p2))` THEN
-    SRW_TAC [][] THEN
-    Q.ISPEC_THEN `q1` (REPEAT_TCL STRIP_THM_THEN SUBST_ALL_TAC)
-                 path_cases THEN
-    Q.ISPEC_THEN `q2` (REPEAT_TCL STRIP_THM_THEN SUBST_ALL_TAC)
-                 path_cases THEN FULL_SIMP_TAC (srw_ss()) []
-    THENL [
-      METIS_TAC [hnf_no_head_redex],
-      METIS_TAC [hnf_no_head_redex],
-      METIS_TAC [is_head_redex_unique, labelled_redn_det]
-    ]
-  ]);
-
-val head_reduction_path_def = new_specification(
-  "head_reduction_path_def",
-  ["head_reduction_path"],
-  CONJUNCT1 ((SIMP_RULE bool_ss [EXISTS_UNIQUE_THM] o
-              SIMP_RULE bool_ss [UNIQUE_SKOLEM_THM])
-             head_reduction_path_uexists));
-
-val head_reduction_path_unique = store_thm(
-  "head_reduction_path_unique",
-  ``!M p. (first p = M) /\ is_head_reduction p /\
-          (finite p ==> hnf (last p)) ==>
-          (head_reduction_path M = p)``,
-  REPEAT STRIP_TAC THEN
-  Q.SPEC_THEN `M` (ASSUME_TAC o CONJUNCT2 o
-                   SIMP_RULE bool_ss [EXISTS_UNIQUE_THM])
-              head_reduction_path_uexists THEN
-  METIS_TAC [head_reduction_path_def]);
-
 val hnf_preserved = store_thm(
   "hnf_preserved",
   ``!M N. reduction beta M N ==> hnf M ==> hnf N``,
@@ -2182,7 +1913,7 @@ Proof
 QED
 
 (* Proposition 8.3.13 (ii) [2, p.174] *)
-Theorem has_hnf_substitutive :
+Theorem has_hnf_if_subst :
     !M. has_hnf ([N/z] M) ==> has_hnf M
 Proof
     Q.X_GEN_TAC ‘M’
